theories/MyRelations.v
@@ -1,6 +1,15 @@
 From Coq Require Import Relations.Relation_Definitions.
 From Coq Require Import Relations.Relation_Operators.
 
+Proposition singlestep_trans (A: Type) (R: relation A):
+  forall x y, R x y -> clos_refl_trans_1n _ R x y.
+Proof.
+  intros.
+  apply rt1n_trans with y.
+  - assumption.
+  - constructor.
+Qed.
+
 Proposition multistep_trans (A: Type) (R: relation A):
   forall x y z, clos_refl_trans_1n _ R x y -> clos_refl_trans_1n _ R y z ->
             clos_refl_trans_1n _ R x z.
