theories/NormalIsomorphism.v
@@ -5,42 +5,9 @@ Require Import Lambda Canonical LambdaIsomorphism.
 From Coq Require Import List Relations.Relation_Definitions.
 Import ListNotations.
 
-Theorem inversion1 :
-  (forall t, Canonical.normal t -> ψ (θ t) = t)
-  /\
-  (forall l, Canonical.normal_list l -> forall s, ψ (θ' s l) = ψ' s l).
-Proof.
-  apply Canonical.mut_normal_ind ; intros ; asimpl ; try easy.
-  - now f_equal. 
-  - fold (θ' (App (Var x) (θ u)) l).
-    fold (ψ (θ' (App (Var x) (θ u)) l)).
-    rewrite H0. asimpl. now f_equal.
-  - fold (θ' (App s (θ u)) l).
-    fold (ψ (θ' (App s (θ u)) l)).
-    rewrite H0. asimpl. now repeat f_equal.
-Qed.
+Definition irreducible s := ~exists s', Lambda.step s s'.
 
-Theorem inversion2 :
-  (forall s, Lambda.normal s -> θ (ψ s) = s)
-  /\
-  (forall a, Lambda.apps a -> forall l, θ (ψ' a l) = θ' a l).
-Proof.
-  apply Lambda.mut_normal_ind ; intros.
-  - asimpl. now f_equal.
-  - now apply H with (l:=[]).
-  - destruct l ; now asimpl.
-  - asimpl. fold (ψ t).
-    rewrite H. asimpl.
-    fold (θ' (App s (θ (ψ t))) l).
-    now rewrite H0.
-Qed.
-
-(*        Digression:      *)
-(* proof using isomorphism *)
-(* ----------------------- *)
-
-Definition irreducible s := ~exists t, Lambda.step s t.
-
+(* In the text as claim 1. => *)
 Theorem nfs_are_irreducible :
   (forall s, Lambda.normal s -> irreducible s)
   /\
@@ -49,23 +16,24 @@ Proof.
   apply Lambda.mut_normal_ind ; intros.
   - intro.
     apply H.
-    destruct H0 as [t Ht].
-    inversion Ht.
+    destruct H0 as [s0 Hs0].
+    inversion Hs0.
     now exists s'.
     - intro.
       apply H.
-      destruct H0 as [t Ht].
-      now exists t.
+      destruct H0 as [s0 Hs0].
+      now exists s0.
     - intro.
       now destruct H.
     - intro.
-      destruct H1 as [t0 Ht0].
-      inversion Ht0 ; subst.
+      destruct H1 as [s0 Hs0].
+      inversion Hs0 ; subst.
       + inversion a.
-      + apply H. now exists s'.
-      + apply H0. now exists t'.
+      + apply H. now exists s1'.
+      + apply H0. now exists s2'.
 Qed.
 
+(* In the text as claim 1. <= *)
 Theorem irreducible_is_nf s :
   irreducible s -> Lambda.normal s.
 Proof.
@@ -88,17 +56,14 @@ Proof.
         eapply Step_App1 in H1. eauto.
     + apply IHs2. intro. apply H.
       inversion H0.
-      apply Step_App2 with (s:=s1) in H1. 
+      apply Step_App2 with (s1:=s1) in H1. 
       now exists (App s1 x).
 Qed.
 
+(* In the text as Claim 4. *)
 Definition irreducible' t := ~exists t', Canonical.step t t'.
-
-Conjecture nts_are_irreducible :
-  forall t, Canonical.normal t -> irreducible' t.
-
-Conjecture irreducible_is_nt :
-  forall t, irreducible' t -> Canonical.normal t.
+Conjecture nts_are_irreducible : forall t, Canonical.normal t -> irreducible' t.
+Conjecture irreducible_is_nt : forall t, irreducible' t -> Canonical.normal t.
 
 Corollary nf_inclusion s :
   Lambda.normal s -> Canonical.normal (ψ s).
